@prefix : <https://w3id.org/oc/ontology#> .
@prefix owl: <http://www.w3.org/2002/07/owl#> .
@prefix rdf: <http://www.w3.org/1999/02/22-rdf-syntax-ns#> .
@prefix xml: <http://www.w3.org/XML/1998/namespace> .
@prefix xsd: <http://www.w3.org/2001/XMLSchema#> .
@prefix rdfs: <http://www.w3.org/2000/01/rdf-schema#> .
@base <https://w3id.org/oc/ontology> .

<https://w3id.org/oc/ontology> rdf:type owl:Ontology ;
                                owl:versionIRI <https://w3id.org/oc/ontology/2019-09-19> .

#################################################################
#    Object Properties
#################################################################

###  https://w3id.org/oc/ontology/contains
<https://w3id.org/oc/ontology/contains> rdf:type owl:ObjectProperty ;
                                        rdfs:domain <https://w3id.org/oc/ontology/InTextReferencePointer> ;
                                        rdfs:range <https://w3id.org/oc/ontology/InTextReferencePointersList> ;
                                        rdfs:comment "The hierarchical relation between elements, e.g. between a list of pointers and each single pointer included in the list." ;
                                        rdfs:label "contains" .


###  https://w3id.org/oc/ontology/denotes
<https://w3id.org/oc/ontology/denotes> rdf:type owl:ObjectProperty ;
                                       rdfs:domain <https://w3id.org/oc/ontology/InTextReferencePointersList> ;
                                       rdfs:range <https://w3id.org/oc/ontology/BibliographicReference> ;
                                       rdfs:comment "The relation between an in-text reference pointer and the bibliographic reference to which it is relevant." ;
                                       rdfs:label "denotes" .


###  https://w3id.org/oc/ontology/hasIdentifier
<https://w3id.org/oc/ontology/hasIdentifier> rdf:type owl:ObjectProperty ;
                                             rdfs:range <https://w3id.org/oc/ontology/Identifier> ;
                                             rdfs:label "has identifier" .


###  https://w3id.org/oc/ontology/hasIdentifierScheme
<https://w3id.org/oc/ontology/hasIdentifierScheme> rdf:type owl:ObjectProperty ;
                                                   rdfs:domain <https://w3id.org/oc/ontology/Identifier> ;
                                                   rdfs:range <https://w3id.org/oc/ontology/IdentifierScheme> ;
                                                   rdfs:label "has identifier scheme" .


###  https://w3id.org/oc/ontology/hasNext
<https://w3id.org/oc/ontology/hasNext> rdf:type owl:ObjectProperty ;
                                       rdfs:comment "The relation between elements in a sequence, e.g. between reference pointers included in a list." ;
                                       rdfs:label "has next" .


###  https://w3id.org/oc/ontology/hasPart
<https://w3id.org/oc/ontology/hasPart> rdf:type owl:ObjectProperty ;
                                       rdfs:domain <https://w3id.org/oc/ontology/Text> ;
                                       rdfs:comment "The hierarchical relation between contents, e.g. texts and bibliographic references." ;
                                       rdfs:label "has part" .


###  https://w3id.org/oc/ontology/references
<https://w3id.org/oc/ontology/references> rdf:type owl:ObjectProperty ;
                                          rdfs:domain <https://w3id.org/oc/ontology/BibliographicReference> ;
                                          rdfs:range <https://w3id.org/oc/ontology/Text> ;
                                          rdfs:comment "The relation between a bibliographic reference and the publication being referenced." ;
                                          rdfs:label "references" .


#################################################################
#    Classes
#################################################################

###  https://w3id.org/oc/ontology/BibliographicReference
<https://w3id.org/oc/ontology/BibliographicReference> rdf:type owl:Class ;
                                                      rdfs:comment "A standard entry in a published work, typically an item within the workâ€™s bibliographic reference list, which refers the reader to an original source of published information referenced or cited by an author in the main body of the text." ,
                                                                   "Bibliographic reference" .


###  https://w3id.org/oc/ontology/Identifier
<https://w3id.org/oc/ontology/Identifier> rdf:type owl:Class ;
                                          rdfs:comment "A string identifying an entity." ;
                                          rdfs:label "Identifier" .


###  https://w3id.org/oc/ontology/IdentifierScheme
<https://w3id.org/oc/ontology/IdentifierScheme> rdf:type owl:Class ;
                                                rdfs:comment "The scheme an identifier conforms to, e.g. XPath syntax." ;
                                                rdfs:label "Identifier scheme" .


###  https://w3id.org/oc/ontology/InTextReferencePointer
<https://w3id.org/oc/ontology/InTextReferencePointer> rdf:type owl:Class ;
                                                      rdfs:comment "A list containing only in-text reference pointers denoting the specific bibliographic references to which the list pertains." ;
                                                      rdfs:label "In-text reference pointers list" .


###  https://w3id.org/oc/ontology/InTextReferencePointersList
<https://w3id.org/oc/ontology/InTextReferencePointersList> rdf:type owl:Class ;
                                                           rdfs:comment "A textual device denoting a single bibliographic reference that is embedded in the text of a document within the context of a particular sentence or text chunk." ;
                                                           rdfs:label "In-text reference pointer" .


###  https://w3id.org/oc/ontology/Text
<https://w3id.org/oc/ontology/Text> rdf:type owl:Class ;
                                    rdfs:comment "The textual content of a published work." ;
                                    rdfs:label "Text" .


###  Generated by the OWL API (version 4.5.9.2019-02-01T07:24:44Z) https://github.com/owlcs/owlapi
